concurrency/Modular/list_inst.v
@@ -19,43 +19,49 @@ Definition t_struct_list_t := Tstruct _list_t noattr.
 
 (* node_rep_R r.1.1.1 r.1.2 r.2 g, and r is type of node_info *)
 #[local]Instance my_specific_tree_rep : NodeRep := {
-  node_rep_R := fun tp r g_info g =>
+    node_rep_R :=
+      fun tp r g_info g =>
+      if eq_dec tp nullval
+      then !!(g_info = Some None) && seplog.emp
+      else (
     EX (gn : gname), EX (x : Z), EX (v next : val), EX (lockn : val),
-      !!(g_info = Some (Some (x, v)) /\ and (Z.le Int.min_signed x) (Z.le x Int.max_signed) /\
+      !!(g_info = Some (Some (x, v, [gn])) /\ and (Z.le Int.min_signed x) (Z.le x Int.max_signed) /\
        is_pointer_or_null next /\ is_pointer_or_null lockn /\
           (tc_val (tptr Tvoid) v) /\ key_in_range x r = true) &&
        data_at Ews t_struct_list ((Vint (Int.repr x)), (v, next)) tp *
        malloc_token Ews t_struct_list tp *
-       in_tree g gn next lockn
+       in_tree g gn next lockn)
 }.
 
+Definition extract_node_gname (node: node_info) : list gname :=
+  match node.2 with
+  | Some (Some (_, _, lst)) => lst
+  | _ => []
+  end.
 
 (* Spec of findnext function *)
 (* FOUND = 0, NOTFOUND = 1, NULLNEXT = 2 (NULLNEXT = NULL || NEXT ) *)
-Check data_at.
-Check data_at Ews (tptr tvoid) (default_val (tptr tvoid)) _.
 
 Definition findnext_spec :=
   DECLARE _findNext
   WITH x: Z, p: val, n: val, n_pt : val, tp: val, r : node_info, g: gname, sh: share, gv: globals
   PRE [ tptr tvoid, tptr (tptr tvoid), tint ]
-          PROP (writable_share sh(*; is_pointer_or_null pa; is_pointer_or_null pb*) )
+          PROP (writable_share sh)
           PARAMS (p; n; Vint (Int.repr x)) GLOBALS (gv)
-          SEP ((* data_at sh (t_struct_tree_t) (p, n) b *)
-            node_rep_R r.1.1.1 r.1.2 r.2 g ;
+          SEP (node_rep_R r.1.1.1 r.1.2 r.2 g ;
                field_at sh (t_struct_list_t) [StructField _t] r.1.1.1 p;
-               data_at sh (tptr t_struct_list_t) n_pt n
-                       (*  *(EX n'', data_at Ews (tptr t_struct_tree_t) n'' n') *) )
+               data_at sh (tptr t_struct_list_t) n_pt n)
   POST [ tint ]
-  EX (stt: enum), EX (n' next : val),
+  EX (stt: enum), EX (n' next : val) (g_in : gname),
          PROP (match stt with
                | F | NF => (n' = p)
                | NN => (n' = next)
                end)
         LOCAL (temp ret_temp (enums stt))
-        SEP (node_rep_R r.1.1.1 r.1.2 r.2 g *
-             field_at sh (t_struct_list_t) [StructField _t] r.1.1.1 p *
-             data_at sh (tptr t_struct_list_t) next n).
+        SEP (!!(g_in ∈ extract_node_gname r) &&
+               node_rep_R r.1.1.1 r.1.2 r.2 g *
+               field_at sh (t_struct_list_t) [StructField _t] r.1.1.1 p *
+               data_at sh (tptr t_struct_list_t) next n).
 
 
 Lemma findNext: semax_body Vprog Gprog f_findNext findnext_spec.
@@ -64,7 +70,13 @@ Proof.
   (* int y = pn->p->t->key *)
   forward. 
   unfold node_rep_R.
-  simpl.
+  destruct (eq_dec r.1.1.1 nullval).
+  + rewrite e.
+    unfold my_specific_tree_rep.
+    rewrite -> if_true; auto.
+    forward.
+    forward.
+    forward.
   Intros gn x0 v0 next lockn.
   forward.
   forward.
@@ -76,23 +88,29 @@ Proof.
     forward. (* t3 = t2->left *)
     forward.
     Exists NN.
-    Exists next next.
+    Exists next next gn.
     entailer !.
-    simpl.
+    unfold extract_node_gname.
+    rewrite H.
+    apply elem_of_list_here.
     Exists gn x0 v0 next lockn.
     entailer !.
   - forward_if.
     (* pn->n = pn->p->t->right *)
     repeat forward.
-    Exists NF p n_pt. simpl.
+    Exists NF p n_pt gn. 
     entailer !.
-    simpl.
+    unfold extract_node_gname.
+    rewrite H.
+    apply elem_of_list_here.
     Exists gn x0 v0 next lockn.
     entailer !.
     forward.
-    Exists F p n_pt.
+    Exists F p n_pt gn.
     entailer !.
-    simpl.
+    unfold extract_node_gname.
+    rewrite H.
+    apply elem_of_list_here.
     Exists gn x0 v0 next lockn.
     entailer !.
 Qed.
